

Convolution theorem corr.

$$\mathcal{L}^{-1} \left\{ \frac{1}{s} F(s) \right\} = \int_0^t f(u) du$$

$$\textcircled{1} \quad \mathcal{L}^{-1} \{ F(s) \} = -\frac{1}{t} \mathcal{L}^{-1} \left\{ \frac{d}{ds} F(s) \right\}$$

Ex ① Find  $\mathcal{L}^{-1} \left\{ \frac{1}{s} \log \left( 1 + \frac{1}{s^2} \right) \right\}$  <sub>16</sub>

$$\textcircled{1} \quad \mathcal{L}^{-1} \left\{ \log \left( 1 + \frac{a^2}{s^2} \right) \right\} \quad \textcircled{11} \quad \mathcal{L}^{-1} \left\{ \log \left( \frac{s+a}{s+b} \right) \right\} \quad \textcircled{13}$$

Soln  $F(s) = \log \left( 1 + \frac{1}{s^2} \right)$

Use  $\mathcal{L}^{-1} \{ F(s) \} = -\frac{1}{t} \mathcal{L}^{-1} \left\{ \frac{d}{ds} F(s) \right\}$

$$= -\frac{1}{t} \mathcal{L}^{-1} \left\{ \frac{d}{ds} \log \left( 1 + \frac{1}{s^2} \right) \right\}$$

$$= -\frac{1}{t} \mathcal{L}^{-1} \left\{ \frac{d}{ds} \log \left( \frac{s^2+1}{s^2} \right) \right\}$$

$$= -\frac{1}{t} \mathcal{L}^{-1} \left\{ \frac{d}{ds} (\log(s^2+1) - \log s^2) \right\}$$

$$= -\frac{1}{t} \mathcal{L}^{-1} \left\{ \frac{d}{ds} \log(s^2+1) - 2 \log s \right\}$$

$$= -\frac{1}{t} \mathcal{L}^{-1} \left\{ \frac{\frac{1}{s^2+1} \cdot 2s}{s^2+1} - \frac{2}{s} \right\}$$

$$= -\frac{2}{t} \left[ \mathcal{L}^{-1} \left\{ \frac{s}{s^2+1} \right\} - \frac{1}{s} \right]$$

$$\mathcal{L}^{-1} \left\{ \log \left( 1 + \frac{1}{s^2} \right) \right\} = -\frac{2}{t} [\cos t - 1] = \frac{2}{t} (1 - \cos t)$$



$$(19) \quad \mathcal{L}^{-1} \left\{ \frac{1}{s} F(s) \right\} = \int_0^t f(u) du$$

$$\therefore \mathcal{L}^{-1} \left\{ \frac{1}{s} \log \left( 1 + \frac{1}{s^2} \right) \right\} = \int_0^t \frac{2}{u} (1 - \cos u) du$$

Ex 2: Find  $\mathcal{L}^{-1} \left\{ \log \left( \frac{s^2+a^2}{s^2+b^2} \right) \right\}$  13.

$$(10) \quad \mathcal{L}^{-1} \left\{ \log \left( \frac{s^2+a^2}{s^2+b^2} \right) \right\} \quad 14$$

Soln (10)  $F(s) = \log \left( \frac{s^2+a^2}{s^2+b^2} \right)$

Use  $\mathcal{L}^{-1} \{ F(s) \} = -\frac{1}{t} \mathcal{L}^{-1} \left\{ \frac{d}{ds} F(s) \right\}$

$$\mathcal{L}^{-1} \left\{ \log \left( \frac{s^2+a^2}{s^2+b^2} \right) \right\} = -\frac{1}{t} \mathcal{L}^{-1} \left\{ \frac{d}{ds} \log \left( \frac{s^2+a^2}{s^2+b^2} \right) \right\}$$

$$= -\frac{1}{t} \mathcal{L}^{-1} \left[ \frac{d}{ds} (\log(s^2+a^2) - \log(s^2+b^2)) \right]$$

$$= -\frac{1}{t} \mathcal{L}^{-1} \left\{ \frac{d}{ds} \log(s^2+a^2) - \frac{d}{ds} \log(s^2+b^2) \right\}$$

$$= -\frac{1}{t} \left[ -\frac{1}{t} \mathcal{L}^{-1} \left\{ \frac{1}{s^2+a^2} \right\} \cdot 2s - \frac{1}{t} \mathcal{L}^{-1} \left\{ \frac{1}{s^2+b^2} \right\} \cdot 2s \right]$$

$$= -\frac{1}{t} \left[ 2 \mathcal{L}^{-1} \left\{ \frac{s}{s^2+a^2} \right\} - \frac{1}{t} \mathcal{L}^{-1} \left\{ \frac{1}{s^2+b^2} \right\} \right]$$

$$= -\frac{1}{t} \left[ 2 \cos at - \frac{1}{2} e^{-bt} \right]$$

$$= \frac{1}{t} \left( \frac{1}{2} e^{-bt} - 2 \cos at \right)$$



(20) Ex (3)  $L^{-1}\left\{\tan^{-1} \frac{a}{s}\right\}$  12, 11  
 $L^{-1}\left\{\cot^{-1}(s+1)\right\}$  76  
 $L^{-1}\left\{\tan^{-1} \frac{s+1}{s}\right\}$  15

Soln  $F(s) = \cot^{-1}(s+1)$

Use  $L^{-1}\{F(s)\} = -\frac{1}{t} L^{-1}\left\{\frac{d}{ds} F(s)\right\}$

$$L^{-1}\left\{\cot^{-1}(s+1)\right\} = -\frac{1}{t} L^{-1}\left\{\frac{d}{ds} \cot^{-1}(s+1)\right\}$$

$$= -\frac{1}{t} L^{-1}\left[-\frac{1}{1+(s+1)^2}\right]$$

$$= \frac{1}{t} L^{-1}\left[\frac{1}{(s+1)^2+1}\right]$$

$$= \frac{1}{t} e^{-t} L^{-1}\left[\frac{1}{s^2+1}\right]$$

$$= \frac{e^{-t}}{t} \sin t$$

HW  $L^{-1}\left\{\cot^{-1}\left(\frac{s+3}{2}\right)\right\}$  ①

Ex (3) Find  $L^{-1}\left\{\tan^{-1} \frac{2}{s^2}\right\}$

Soln  $L^{-1}\{F(s)\} = -\frac{1}{t} L^{-1}\left\{\frac{d}{ds} F(s)\right\}$

$$L^{-1}\left\{\tan^{-1} \frac{2}{s^2}\right\} = -\frac{1}{t} L^{-1}\left\{\frac{d}{ds} \tan^{-1} \frac{2}{s^2}\right\}$$

$$= -\frac{1}{t} \left[ \frac{1}{1+\frac{4}{s^4}} \cdot 2(-2s^{-3}) \right]$$



$$\textcircled{2} \quad \mathcal{L}^{-1} \left\{ \tan^{-1} \frac{2}{s^2} \right\} = -\frac{1}{t} \mathcal{L}^{-1} \left\{ \frac{1}{\frac{s^4+4}{s^4}} \left( -\frac{4}{s^2} \right) \right\}$$

$$= \frac{4}{t} \mathcal{L}^{-1} \left\{ \frac{s}{s^4+4} \right\} \quad \text{--- (1)}$$

$$\text{Let } \frac{s}{s^4+4} = \frac{s}{(s^2+2s+2)(s^2-2s+2)} = \frac{s}{(s^2+2)^2 - (2s)^2}$$

$$= \frac{s}{(s^2-2s+2)(s^2+2s+2)} = \frac{s}{s^2-2s+2} \cdot \frac{1}{s^2+2s+2}$$

$$\text{Let } \frac{1}{S \cdot B} = \frac{1}{B-S} \left( \frac{1}{S} - \frac{1}{B} \right)$$

$$\frac{1}{(s^2-2s+2)(s^2+2s+2)} = \frac{1}{4s} \left( \frac{1}{s^2-2s+2} - \frac{1}{s^2+2s+2} \right)$$

$$\textcircled{2} \quad \frac{1 \cdot s}{(s^2-2s+2)(s^2+2s+2)} = \frac{1s}{4s} \left( \frac{1}{s^2-2s+2} - \frac{1}{s^2+2s+2} \right)$$

$$\text{from (1)} \quad \mathcal{L}^{-1} \left\{ \frac{s}{s^4+4} \right\} = \frac{1}{4} \mathcal{L}^{-1} \left\{ \frac{1}{s^2-2s+2} - \frac{1}{s^2+2s+2} \right\}$$

$$= \frac{1}{4} \left[ \mathcal{L}^{-1} \left\{ \frac{1}{s^2-2s+2} \right\} - \mathcal{L}^{-1} \left\{ \frac{1}{s^2+2s+2} \right\} \right]$$

$$= \frac{1}{4} \left[ \mathcal{L}^{-1} \left\{ \frac{1}{(s-1)^2+1} \right\} - \mathcal{L}^{-1} \left\{ \frac{1}{(s+1)^2+1} \right\} \right]$$

$$= \frac{1}{4} [e^t \sin t - e^{-t} \sin t] =$$

$$= \frac{1}{2} \sin t \left( \frac{e^t - e^{-t}}{2} \right) = \frac{1}{2} \sin t \sinh t$$

from (1)

$$= \frac{4}{t} \cdot \frac{1}{2} \sin t \sinh t = \frac{2}{t} \sin t \sinh t$$



Q2) Use convolution thm PT.

$$\mathcal{L}^{-1}\left\{\frac{1}{s} \log\left(\frac{s+a}{s+b}\right)\right\} = \int_0^t \frac{e^{-bu} - e^{-au}}{u} du \quad 13$$

Soln (i)  $\mathcal{L}^{-1}\left\{\frac{1}{s} \tan^{-1}\left(\frac{s+a}{b}\right)\right\} = \int_0^t -\frac{1}{u} e^{-au} \sin bu \, du$

Soln (ii)  $F(s) = \tan^{-1}\left(\frac{s+a}{b}\right)$

$$\mathcal{L}^{-1}\{F(s)\} = -\frac{1}{t} \mathcal{L}^{-1}\left\{\frac{d}{ds} F(s)\right\}$$

$$\mathcal{L}^{-1}\left\{\tan^{-1}\left(\frac{s+a}{b}\right)\right\} = -\frac{1}{t} \mathcal{L}^{-1}\left\{\frac{d}{ds} \tan^{-1}\left(\frac{s+a}{b}\right)\right\}$$

$$= -\frac{1}{t} \mathcal{L}^{-1}\left\{\frac{1}{1 + \frac{(s+a)^2}{b^2}} \cdot \frac{1}{b} \cdot 1\right\}$$

$$= -\frac{1}{t} \mathcal{L}^{-1}\left\{\frac{b^2}{(s+a)^2 + b^2} \cdot \frac{1}{b}\right\}$$

$$= -\frac{b}{t} \mathcal{L}^{-1}\left\{\frac{1}{(s+a)^2 + b^2}\right\}$$

$$= -\frac{b}{t} e^{-at} \mathcal{L}^{-1}\left\{\frac{1}{s^2 + b^2}\right\}$$

$$= -\frac{b}{t} \cdot \frac{1}{b} e^{-at} \sin bt$$

$$= -\frac{1}{t} e^{-at} \sin bt = f(u)$$

$$\mathcal{L}^{-1}\left\{\frac{1}{s} \tan^{-1}\left(\frac{s+a}{b}\right)\right\} = \int_0^t f(u) \, du$$

$$= - \int_0^t \frac{1}{u} e^{-au} \sin bu \, du$$

$$= - \int_0^t \frac{1}{u} e^{-au} \sin bu \, du$$